theories/case_studies/macros/assert_spec.v
@@ -1,0 +1,213 @@
+From iris.proofmode Require Import proofmode.
+From cap_machine Require Import logrel rules proofmode.
+From cap_machine Require Import fetch_spec.
+From cap_machine Require Export assert.
+
+(* Assert routine *)
+
+(* Maintains a flag storing whether an assert has failed. *)
+
+Section Assert_subroutine.
+  Context
+    {Σ : gFunctors}
+      {ceriseg: ceriseG Σ}
+      {nainv: logrel_na_invs Σ}
+      {MP: MachineParameters}
+  .
+
+  (* Asserts (ct0 == ct1). Jumps back to cra.
+     Clobbers cra, ct0, ct1.
+   *)
+  Definition assert_subroutine_instrs :=
+    encodeInstrsW [
+      Sub ct0 ct0 ct1;
+      Jnz 4 ct0;
+      (* success case *)
+      Mov ct0 0;
+      Mov ct1 0;
+      JmpCap cra; (* return *)
+      (* failure case *)
+      Mov ct1 PC; (* pointer to cap: *)
+      Lea ct1 7; (* pointer to cap: *)
+      Load ct1 ct1;
+      Store ct1 1;
+      Mov ct0 0;
+      Mov ct1 0;
+      JmpCap cra (* return *)
+    ].
+  (* followed in memory by:
+    cap: (RW, flag, end, flag)
+    flag: <0 or 1>
+    end:
+  *)
+
+  Definition assert_inv (b_assert e_assert a_flag : Addr) : iProp Σ :=
+    (∃ cap_addr,
+       codefrag b_assert assert_subroutine_instrs ∗
+       ⌜(b_assert + length assert_subroutine_instrs)%a = Some cap_addr⌝ ∗
+       ⌜(cap_addr + 1)%a = Some e_assert⌝ ∗
+       ⌜is_Some (a_flag + 1)%a⌝ ∗
+       cap_addr ↦ₐ WCap RW Global a_flag (a_flag ^+1)%a a_flag).
+
+  Lemma assert_subroutine_spec
+    (pc_g : Locality) (pc_b pc_e a_flag : Addr)
+    ( n1 n2 flag : Z ) ( wret : Word)
+    (N : namespace) (E : coPset) (φ : language.val cap_lang -> iProp Σ) :
+    ↑N ⊆ E →
+    (  na_inv logrel_nais N (assert_inv pc_b pc_e a_flag)
+     ∗ na_own logrel_nais E
+     ∗ PC ↦ᵣ WCap RX pc_g pc_b pc_e pc_b
+     ∗ cra ↦ᵣ wret
+     ∗ ct0 ↦ᵣ WInt n1
+     ∗ ct1 ↦ᵣ WInt n2
+     ∗ a_flag ↦ₐ WInt flag
+     ∗ ▷ (na_own logrel_nais E
+          ∗ PC ↦ᵣ updatePcPerm wret
+          ∗ cra ↦ᵣ wret
+          ∗ ct0 ↦ᵣ WInt 0
+          ∗ ct1 ↦ᵣ WInt 0
+          ∗ a_flag ↦ₐ WInt (if (n1 =? n2)%Z then flag else 1%Z)
+          -∗ WP Seq (Instr Executable) {{ φ }})
+     ⊢ WP Seq (Instr Executable) {{ φ }})%I.
+  Proof.
+    iIntros (HNE) "(#Hinv & Hna & HPC & Hrdst & Hct0 & Hct1 & Hflag & Hφ)".
+    iMod (na_inv_acc with "Hinv Hna") as "(>Hassert & Hna & Hinv_close)"; auto.
+    iDestruct "Hassert" as (cap_addr) "(Hprog & %Hcap & %Hpc_e & %He_flag & Hcap)".
+    destruct He_flag as [e_flag He_flag].
+    rewrite /assert_subroutine_instrs.
+    codefrag_facts "Hprog". rename H into HcontProg.
+    assert (SubBounds pc_b pc_e
+              pc_b (pc_b ^+ length assert_subroutine_instrs)%a)
+      as HsubBounds by solve_addr.
+    iInstr "Hprog".
+    destruct (decide (n1 = n2)) as [Heq|Heq].
+    { (* n1 = n2 *)
+      subst n2. rewrite (_: n1 - n1 = 0)%Z; last lia.
+      iGo "Hprog".
+      iMod ("Hinv_close" with "[Hprog Hcap $Hna]") as "Hna".
+      { iExists _. iNext. iFrame. iPureIntro. repeat split; solve_addr. }
+
+      iApply "Hφ". iFrame. rewrite Z.eqb_refl //. }
+    { (* n1 ≠ n2 *)
+      iInstr "Hprog". { assert (n1 - n2 ≠ 0)%Z by lia. congruence. }
+      iInstr "Hprog".
+      iInstr "Hprog".
+      rewrite (_: (pc_b ^+ 12)%a = cap_addr); [|solve_addr].
+      iInstr "Hprog"; first solve_addr.
+      iInstr "Hprog"; first solve_addr.
+      iGo "Hprog".
+      iMod ("Hinv_close" with "[Hprog Hcap $Hna]") as "Hna".
+      { iExists _. iNext. iFrame. iPureIntro. repeat split; solve_addr. }
+      iApply "Hφ". iFrame. rewrite (_: (n1 =? n2)%Z = false) //.
+      by apply Z.eqb_neq. }
+  Qed.
+
+  Lemma assert_subroutine_success_spec
+    (pc_g : Locality) (pc_b pc_e a_flag : Addr)
+    ( n1 n2 flag : Z ) ( wret : Word)
+    (N : namespace) (E : coPset) (φ : language.val cap_lang -> iProp Σ) :
+    ↑N ⊆ E →
+    n1 = n2 →
+    (  na_inv logrel_nais N (assert_inv pc_b pc_e a_flag)
+     ∗ na_own logrel_nais E
+     ∗ PC ↦ᵣ WCap RX pc_g pc_b pc_e pc_b
+     ∗ cra ↦ᵣ wret
+     ∗ ct0 ↦ᵣ WInt n1
+     ∗ ct1 ↦ᵣ WInt n2
+     ∗ ▷ (na_own logrel_nais E
+          ∗ PC ↦ᵣ updatePcPerm wret
+          ∗ cra ↦ᵣ wret
+          ∗ ct0 ↦ᵣ WInt 0%Z
+          ∗ ct1 ↦ᵣ WInt 0%Z
+          -∗ WP Seq (Instr Executable) {{ φ }})
+     ⊢ WP Seq (Instr Executable) {{ φ }})%I.
+  Proof.
+    iIntros (HNE Heq) "(#Hinv & Hna & HPC & Hrdst & Hct0 & Hct1 & Hφ)".
+    iMod (na_inv_acc with "Hinv Hna") as "(>Hassert & Hna & Hinv_close)"; auto.
+    iDestruct "Hassert" as (cap_addr) "(Hprog & %Hcap & %Hflag & %He & Hcap)".
+    rewrite /assert_subroutine_instrs. codefrag_facts "Hprog".
+    assert (SubBounds pc_b pc_e
+              pc_b (pc_b ^+ length assert_subroutine_instrs)%a)
+      as HsubBounds by solve_addr.
+    iInstr "Hprog".
+    rewrite (_: n1 - n2 = 0)%Z; last lia.
+    iGo "Hprog".
+    iMod ("Hinv_close" with "[Hprog Hcap $Hna]") as "Hna".
+    { iExists _. iNext. iFrame. iPureIntro. repeat split; solve_addr. }
+    iApply "Hφ". iFrame.
+  Qed.
+
+End Assert_subroutine.
+
+Section Assert.
+  Context
+    {Σ : gFunctors}
+      {ceriseg: ceriseG Σ}
+      {nainv: logrel_na_invs Σ}
+      {MP: MachineParameters}
+  .
+
+  Lemma assert_success_spec
+    (n : Z) (rdst rscratch1 rscratch2 : RegName)
+    (pc_g : Locality) (pc_p : Perm) (pc_b pc_e pc_a : Addr)
+    (g_assert : Locality) (b_assert e_assert a_flag : Addr)
+    (n1 n2 : Z) (wdst wcra w1 w2 : Word)
+    (N : namespace) (E : coPset) (φ : language.val cap_lang -> iProp Σ) :
+
+    let assert_macro := assert_instrs n rdst rscratch1 rscratch2 in
+    let a_last := (pc_a ^+ length assert_macro)%a in
+    executeAllowed pc_p = true →
+    SubBounds pc_b pc_e pc_a a_last →
+    withinBounds pc_b pc_e (pc_b ^+ n)%a = true ->
+
+    ↑N ⊆ E →
+    n1 = n2 →
+    (  na_inv logrel_nais N (assert_inv b_assert e_assert a_flag)
+     ∗ na_own logrel_nais E
+     ∗ PC ↦ᵣ WCap pc_p pc_g pc_b pc_e pc_a
+     ∗ rdst ↦ᵣ wdst
+     ∗ rscratch1 ↦ᵣ w1
+     ∗ rscratch2 ↦ᵣ w2
+     ∗ cra ↦ᵣ wcra
+     ∗ ct0 ↦ᵣ WInt n1
+     ∗ ct1 ↦ᵣ WInt n2
+     ∗ codefrag pc_a assert_macro
+     ∗ (pc_b ^+ n)%a ↦ₐ (WSentry RX g_assert b_assert e_assert b_assert)
+     ∗ ▷ (na_own logrel_nais E
+          ∗ PC ↦ᵣ WCap pc_p pc_g pc_b pc_e a_last
+          ∗ rdst ↦ᵣ WInt 0
+          ∗ rscratch1 ↦ᵣ WInt 0
+          ∗ rscratch2 ↦ᵣ WInt 0
+          ∗ cra ↦ᵣ wcra
+          ∗ ct0 ↦ᵣ WInt 0
+          ∗ ct1 ↦ᵣ WInt 0
+          ∗ codefrag pc_a assert_macro
+          ∗ (pc_b ^+ n)%a ↦ₐ (WSentry RX g_assert b_assert e_assert b_assert)
+          -∗ WP Seq (Instr Executable) {{ φ }})
+     ⊢ WP Seq (Instr Executable) {{ φ }})%I.
+  Proof.
+    intros assert_macro a_last; subst assert_macro a_last.
+    iIntros (Hpc_exec HsubBounds Hinbounds HNE Heq)
+      "(#Hinv & Hna & HPC & Hrdst & Hrscratch1 & Hrscratch2 & Hcra & Hct0 & Hct1 & Hcode & Hpc_bn & Hφ)".
+    codefrag_facts "Hcode".
+    rewrite /assert_instrs /assembled_assert.
+    repeat (iEval (cbn [concat]) in "Hcode").
+    repeat (iEval (cbn [fmap list_fmap]) in "Hcode").
+    focus_block_0 "Hcode" as "Hfetch" "Hcont".
+    iApply (fetch_spec with "[-]"); eauto; iFrame.
+    iNext; iIntros "(HPC & Hrdst & Hrscratch1 & Hrscratch2 & Hfetch & Hpc_bn)".
+    unfocus_block "Hfetch" "Hcont" as "Hcode".
+    focus_block 1 "Hcode" as a_assert Ha_assert "Hassert" "Hcont".
+    iGo "Hassert".
+    rewrite load_word_sentry.
+    iEval (cbn) in "HPC".
+    iApply (assert_subroutine_success_spec with "[-]"); eauto; iFrame "#∗".
+    iNext; iIntros "(Hna & HPC & Hcra & Hct0 & Hct1)".
+    iEval (cbn) in "HPC".
+    iGo "Hassert".
+    unfocus_block "Hassert" "Hcont" as "Hcode".
+    replace (a_assert ^+ 5)%a with (pc_a ^+ 14)%a by solve_addr.
+    iApply "Hφ"; iFrame.
+  Qed.
+
+End Assert.
